theories/Dijkstra/DelaySpecMonad.v
@@ -1,0 +1,171 @@
+From Coq Require Import
+     Arith.PeanoNat
+     Lists.List
+     Strings.String
+     Morphisms
+     Setoid
+     RelationClasses
+     Logic.Classical_Prop
+.
+
+From ExtLib Require Import
+     Data.String
+     Structures.Monad
+     Structures.Traversable
+     Data.List.
+
+From ITree Require Import
+     ITree
+     ITreeFacts
+     Events.MapDefault
+     Events.State
+     Events.StateFacts
+     Core.Divergence
+     Dijkstra.DijkstraMonad
+     Dijkstra.PureITreeBasics
+   (*  Simple *)
+.
+
+From Paco Require Import paco.
+
+Import Monads.
+Import MonadNotation.
+Local Open Scope monad_scope.
+
+Ltac clear_ret_eutt_spin :=
+  match goal with | H : ret ?a ≈ spin  |- _ => simpl in H; exfalso; eapply not_ret_eutt_spin; eauto
+             | H : Ret ?a ≈ spin  |- _ => exfalso; eapply not_ret_eutt_spin; eauto
+             | H : spin ≈ ret ?a  |- _ => exfalso; symmetry in H; eapply not_ret_eutt_spin; eauto
+             | H : divergence (ret _ ) |- _ => pinversion H
+  end.
+  
+Ltac invert_evidence :=
+  intros; repeat match goal with 
+                 | H : _ /\ _ |- _ => destruct H
+                 | H : _ \/ _ |- _ => destruct H 
+                 | H : exists a : ?A, _ |- _ => destruct H as [?a ?H]
+                 | x : ?A + ?B |- _ => destruct x as [?a | ?b]
+                 | H : upaco1 _ _ _ |- _ => pclearbot
+                 end.
+
+Ltac invert_ret := simpl in *; match goal with | H : Ret ?a ≈ Ret ?b |- _ => 
+                                                 apply inv_ret in H; try discriminate; try (injection H as H);
+                                                 subst end.
+
+
+Ltac basic_solve := invert_evidence; try clear_ret_eutt_spin; try invert_ret.
+
+Ltac dest_dep f a := destruct (f a) as [?fa ?Hfa] eqn : ?Heq; simpl in *.
+
+
+Notation "a ∈ b" := (proj1_sig b a) (at level 70). 
+
+Notation "a ∋ b" := (proj1_sig a b) (at level 70).
+
+Definition Delay (A : Type) := itree Void A.
+
+Global Instance EqMDelay : EqM Delay := @ITreeMonad.EqM_ITree Void.
+
+Global Instance MonadDelay : Monad Delay := @Monad_itree Void.
+
+Definition DelaySpecInput (A : Type) := {p : Delay A -> Prop | resp_eutt _ _ p}.
+
+Definition DelayIn {A : Type} (t : Delay A) (p : DelaySpecInput A) := proj1_sig p t.
+
+Definition DelaySpec (A : Type) := {w : DelaySpecInput A -> Prop | forall (p p' : DelaySpecInput A),
+                                   (forall t, t ∈ p -> t ∈ p') -> w p -> w p'}.
+
+Program Definition ret_del (A : Type) (a : A) : DelaySpec A := fun p => p (Ret a).
+
+
+Program Definition _bind_del (A B : Type) (w : DelaySpec A) (f : A -> DelaySpec B):=
+  fun p => w ∋ (fun t => (exists a, Ret a ≈ t /\ p ∈ f a) \/ (divergence t /\ p spin)).
+Next Obligation.
+  intros t1 t2 Heutt. split; intros; basic_solve.
+  - left. exists a. split; auto. rewrite H. auto.
+  - right. rewrite <- Heutt. auto.
+  - left. exists a. rewrite Heutt. auto.
+  - right. rewrite Heutt. auto.
+Qed.
+
+Program Definition bind_del (A B : Type) (w : DelaySpec A) (f : A -> DelaySpec B) : DelaySpec B :=
+  _bind_del A B w f.
+Next Obligation.
+  red. red in H0. destruct w as [w Hw]. simpl in *. eapply Hw; try apply H0.
+  simpl. intros. basic_solve.
+  - left. exists a. split; auto. dest_dep f a. eapply Hfa; eauto.
+  - right. split; auto.
+Qed.
+
+Global Instance DelaySpecEq : EqM DelaySpec :=
+  fun _ w1 w2 => forall p, p ∈ w1 <-> p ∈ w2.
+
+Global Instance DelaySpecMonad : Monad DelaySpec :=
+  {
+    ret := ret_del;
+    bind := bind_del
+  }.
+
+Program Instance DelaySpecMonadLaws : MonadLaws DelaySpec.
+Next Obligation.
+  repeat red. cbn. split; intros; basic_solve; auto.
+  - pinversion H.
+  - left. exists x. split; auto; reflexivity.
+Qed.
+Next Obligation.
+  rename a into A.
+  rename x into w.
+  repeat red. cbn. split; intros.
+  - red in H. simpl in H. destruct w as [w Hw]. simpl in *. eapply Hw; try apply H.
+    intros. simpl in *. destruct p as [p Hp]. simpl in *. basic_solve.
+    +  eapply Hp; eauto. symmetry. auto.
+    + apply div_spin_eutt in H0. eapply Hp; eauto.
+  - red. destruct w as [w Hw]. simpl in *. eapply Hw; try apply H. intros.
+    destruct p as [p Hp]. simpl in *.
+    destruct (eutt_reta_or_div _ t); basic_solve. 
+    + left. exists a. split; auto. eapply Hp; eauto.
+    + right. split; auto. eapply Hp; try apply H0. symmetry. apply div_spin_eutt. auto.
+Qed.
+Next Obligation.
+  rename a into A. rename b into B. rename c into C. rename x into w.
+  repeat red. cbn. split; intros. 
+  - red. red in H. destruct w as [w Hw]. simpl in *. destruct p as [p Hp]. simpl in *.
+    eapply Hw; try apply H. intros. simpl in *. clear H. basic_solve.
+    + left. exists a. auto.
+    + right. auto.
+  - red. red in H. destruct w as [w Hw]. simpl in *. destruct p as [p Hp]. simpl in *.
+    eapply Hw; try apply H. simpl in *. intros. basic_solve.
+    + left. exists a. auto.
+    + right. split; auto. right. split; try auto using spin_div.
+Qed.
+
+Global Instance DelaySpecOrderM : OrderM DelaySpec :=
+  fun _ w1 w2 => forall p, p ∈ w2 -> p ∈ w1.
+
+Global Instance DelaySpecOrder : OrderedMonad DelaySpec.
+Proof.
+  red. intros. repeat red. cbn. destruct w1 as [w1 Hw1]. destruct w2 as [w2 Hw2].
+  intros. simpl in *. apply H. simpl in *. eapply Hw2; try apply H1. simpl in *. intros.
+  basic_solve.
+  - left. exists a. split; auto. apply H0. auto.
+  - right. auto.
+Qed.
+
+Program Definition obs_del (A : Type) (t : Delay A) : DelaySpec A := fun p => t ∈ p.
+
+Global Instance DelaySpecObs : EffectObs Delay DelaySpec := obs_del.
+
+Global Instance DelaySpecMonadMorph : MonadMorphism Delay DelaySpec DelaySpecObs.
+Proof.
+  constructor.
+  - repeat red. cbn. tauto.
+  - repeat red. cbn. split; intros; basic_solve.
+    + destruct (eutt_reta_or_div _ m); basic_solve.
+      * left. exists a. split; auto. destruct p as [p Hp]. simpl in *. eapply Hp; try apply H.
+        rewrite <- H0. setoid_rewrite bind_ret. reflexivity.
+      * right. split; auto. apply div_spin_eutt in H0. destruct p as [p Hp]. eapply Hp; try apply H.
+        rewrite H0. apply spin_bind.
+    + destruct p as [p Hp]. simpl in *. eapply Hp; try apply H0. rewrite <- H. setoid_rewrite bind_ret. reflexivity.
+    + apply div_spin_eutt in H. destruct p as [p Hp]. simpl in *. eapply Hp; try apply H0. rewrite H. 
+      symmetry. apply spin_bind.
+Qed.
