theories/Dijkstra/StateSpecT.v
@@ -1,0 +1,75 @@
+From Coq Require Import
+     Arith.PeanoNat
+     Lists.List
+     Strings.String
+     Morphisms
+     Setoid
+     RelationClasses
+     Logic.Classical_Prop
+.
+
+From ExtLib Require Import
+     Data.String
+     Structures.Monad
+     Structures.Traversable
+     Data.List.
+
+From ITree Require Import
+     ITree
+     ITreeFacts
+     Events.MapDefault
+     Events.State
+     Events.StateFacts
+     Core.Divergence
+     Dijkstra.DijkstraMonad
+     Dijkstra.PureITreeBasics
+   (*  Simple *)
+.
+
+From Paco Require Import paco.
+
+Import Monads.
+Import MonadNotation.
+Local Open Scope monad_scope.
+
+Ltac clear_ret_eutt_spin :=
+  match goal with | H : ret ?a ≈ spin  |- _ => simpl in H; exfalso; eapply not_ret_eutt_spin; eauto
+             | H : Ret ?a ≈ spin  |- _ => exfalso; eapply not_ret_eutt_spin; eauto
+             | H : spin ≈ ret ?a  |- _ => exfalso; symmetry in H; eapply not_ret_eutt_spin; eauto
+             | H : divergence (ret _ ) |- _ => pinversion H
+  end.
+  
+Ltac invert_evidence :=
+  intros; repeat match goal with 
+                 | H : _ /\ _ |- _ => destruct H
+                 | H : _ \/ _ |- _ => destruct H 
+                 | H : exists a : ?A, _ |- _ => destruct H as [?a ?H]
+                 | x : ?A + ?B |- _ => destruct x as [?a | ?b]
+                 | H : upaco1 _ _ _ |- _ => pclearbot
+                 end.
+
+Ltac invert_ret := simpl in *; match goal with | H : Ret ?a ≈ Ret ?b |- _ => 
+                                                 apply inv_ret in H; try discriminate; try (injection H as H);
+                                                 subst end.
+
+
+Ltac basic_solve := invert_evidence; try clear_ret_eutt_spin; try invert_ret.
+
+Ltac dest_dep f a := destruct (f a) as [?fa ?Hfa] eqn : ?Heq; simpl in *.
+
+
+Notation "a ∈ b" := (proj1_sig b a) (at level 70). 
+
+Notation "a ∋ b" := (proj1_sig a b) (at level 70).
+
+Section StateSpecT.
+  Context (S : Type).
+  Context (W : Type -> Type).
+
+  Context {SpecMonadW : SpecMonad W}.
+
+  Definition StateSpecT (A : Type) := S -> Input W (S *A) -> Prop.
+
+End StateSpecT.
+
+
